Liveness.v
@@ -30,117 +30,76 @@ Definition isImperative (o:overapproximation) :=
 
 (** ** Inductive Definition of Liveness *)
 
-Inductive live_sound (i:overapproximation) : list (set var*params) -> stmt -> ann (set var) -> Prop :=
-| LOpr x Lv b lv e (al:ann (set var))
-  :  live_sound i Lv b al
-  -> live_exp_sound e lv
-  -> (getAnn al\ singleton x) ⊆ lv
-  -> x ∈ getAnn al
-  -> live_sound i Lv (stmtLet x e b) (ann1 lv al)
-| LIf Lv e b1 b2 lv al1 al2
-  :  live_sound i Lv b1 al1
-  -> live_sound i Lv b2 al2
-  -> live_exp_sound e lv
-  -> getAnn al1 ⊆ lv
-  -> getAnn al2 ⊆ lv
-  -> live_sound i Lv (stmtIf e b1 b2) (ann2 lv al1 al2)
-| LGoto l Y Lv lv blv Z
-  : get Lv (counted l) (blv,Z) (** Imperative Liveness requires the globals of a function to be live at the call site *)
-  -> (if isImperative i then ((blv \ of_list Z) ⊆ lv) else True)
-  -> length Y = length Z
-  -> (forall n y, get Y n y -> live_exp_sound y lv)
-  -> live_sound i Lv (stmtApp l Y) (ann0 lv)
-| LReturn Lv e lv
+Inductive live_sound (i:overapproximation)
+  : list params -> list (set var) -> stmt -> ann (set var) -> Prop :=
+| LOpr ZL Lv x e s lv (al:ann (set var))
+  :  live_sound i ZL Lv s al
+     -> live_exp_sound e lv
+     -> (getAnn al \ singleton x) ⊆ lv
+     -> x ∈ getAnn al
+     -> live_sound i ZL Lv (stmtLet x e s) (ann1 lv al)
+| LIf Lv ZL e s1 s2 lv al1 al2
+  :  live_sound i ZL Lv s1 al1
+     -> live_sound i ZL Lv s2 al2
+     -> live_exp_sound e lv
+     -> getAnn al1 ⊆ lv
+     -> getAnn al2 ⊆ lv
+     -> live_sound i ZL Lv (stmtIf e s1 s2) (ann2 lv al1 al2)
+| LGoto ZL Lv l Y lv blv Z
+  : get ZL (counted l) Z
+    -> get Lv (counted l) blv
+    (** Imperative Liveness requires the globals of a function to be live at the call site *)
+    -> (if isImperative i then ((blv \ of_list Z) ⊆ lv) else True)
+    -> length Y = length Z
+    -> (forall n y, get Y n y -> live_exp_sound y lv)
+    -> live_sound i ZL Lv (stmtApp l Y) (ann0 lv)
+| LReturn ZL Lv e lv
   : live_exp_sound e lv
-  -> live_sound i Lv (stmtReturn e) (ann0 lv)
-| LExtern x Lv b lv Y al f
-  :  live_sound i Lv b al
-  -> (forall n y, get Y n y -> live_exp_sound y lv)
-  -> (getAnn al\ singleton x) ⊆ lv
-  -> x ∈ getAnn al
-  -> live_sound i Lv (stmtExtern x f Y b) (ann1 lv al)
-| LLet Lv F b lv als alb
-  : live_sound i (zip pair (getAnn ⊝ als) (fst ⊝ F) ++ Lv) b alb
+    -> live_sound i ZL Lv (stmtReturn e) (ann0 lv)
+| LExternZL ZL Lv x f Y s lv al
+  :  live_sound i ZL Lv s al
+     -> (forall n y, get Y n y -> live_exp_sound y lv)
+     -> (getAnn al \ singleton x) ⊆ lv
+     -> x ∈ getAnn al
+     -> live_sound i ZL Lv (stmtExtern x f Y s) (ann1 lv al)
+| LLet ZL Lv F t lv als alb
+  : live_sound i (fst ⊝ F ++ ZL) (getAnn ⊝ als ++ Lv) t alb
     -> length F = length als
-  -> (forall n Zs a, get F n Zs ->
-               get als n a ->
-               live_sound i (zip pair (getAnn ⊝ als) (fst ⊝ F) ++ Lv) (snd Zs) a)
-  -> (forall n Zs a, get F n Zs ->
-               get als n a ->
-               (of_list (fst Zs)) ⊆ getAnn a
-               /\ (if isFunctional i then (getAnn a \ of_list (fst Zs)) ⊆ lv else True))
-  -> getAnn alb ⊆ lv
-  -> live_sound i Lv (stmtFun F b)(annF lv als alb).
+    -> (forall n Zs a, get F n Zs ->
+                 get als n a ->
+                 live_sound i (fst ⊝ F ++ ZL) (getAnn ⊝ als ++ Lv) (snd Zs) a)
+    -> (forall n Zs a, get F n Zs ->
+                 get als n a ->
+                 (of_list (fst Zs)) ⊆ getAnn a
+                 /\ (if isFunctional i then (getAnn a \ of_list (fst Zs)) ⊆ lv else True))
+    -> getAnn alb ⊆ lv
+    -> live_sound i ZL Lv (stmtFun F t)(annF lv als alb).
 
 
 (** ** Relation between different overapproximations *)
 
-Lemma live_sound_overapproximation_I Lv s slv
-: live_sound FunctionalAndImperative Lv s slv -> live_sound Imperative Lv s slv.
+Lemma live_sound_overapproximation_I ZL Lv s slv
+: live_sound FunctionalAndImperative ZL Lv s slv -> live_sound Imperative ZL Lv s slv.
 Proof.
   intros. general induction H; simpl in * |- *; econstructor; simpl; eauto.
   - intros. edestruct H3; eauto.
 Qed.
 
-Lemma live_sound_overapproximation_F Lv s slv
-: live_sound FunctionalAndImperative Lv s slv -> live_sound Functional Lv s slv.
+Lemma live_sound_overapproximation_F ZL Lv s slv
+: live_sound FunctionalAndImperative ZL Lv s slv -> live_sound Functional ZL Lv s slv.
 Proof.
   intros. general induction H; simpl in * |- *; econstructor; simpl; eauto.
 Qed.
 
 (** ** [live_sound] ensures that the annotation matches the program *)
-Lemma live_sound_annotation i Lv s slv
-: live_sound i Lv s slv -> annotation s slv.
+Lemma live_sound_annotation i ZL Lv s slv
+: live_sound i ZL Lv s slv -> annotation s slv.
 Proof.
   intros. general induction H; econstructor; eauto.
 Qed.
 
 (** ** Some monotonicity properties *)
 
-Definition live_ann_subset (lvZ lvZ' : set var * list var) :=
-  match lvZ, lvZ' with
-    | (lv,Z), (lv',Z') => lv' ⊆ lv /\ Z = Z'
-  end.
-
-Instance live_ann_subset_refl : Reflexive live_ann_subset.
-hnf; intros. destruct x; firstorder.
-Qed.
-
-Lemma live_sound_monotone i LV LV' s lv
-: live_sound i LV s lv
-  -> PIR2 live_ann_subset LV LV'
-  -> live_sound i LV' s lv.
-Proof.
-  intros. general induction H; simpl; eauto using live_sound.
-  - edestruct PIR2_nth; eauto; dcr; simpl in *.
-    destruct x; subst; simpl in *.
-    econstructor; eauto.
-    cases; simpl in *; eauto; dcr; subst.
-    rewrite <- H0. rewrite <- H4. reflexivity.
-    cset_tac; eauto.
-  - econstructor; eauto 20 using PIR2_app.
-Qed.
-
-Lemma live_sound_monotone2 i LV s lv a
-: live_sound i LV s lv
-  -> getAnn lv ⊆ a
-  -> live_sound i LV s (setTopAnn lv a).
-Proof.
-  intros. general induction H; simpl in * |- *; eauto using live_sound, live_exp_sound, Subset_trans.
-  - econstructor; eauto using live_exp_sound_incl.
-    etransitivity; eauto.
-  - econstructor; eauto using live_exp_sound_incl; etransitivity; eauto.
-  - econstructor; eauto using live_exp_sound_incl.
-    destruct i; simpl; eauto; rewrite <- H3; eauto.
-  - econstructor; eauto using live_exp_sound_incl; etransitivity; eauto.
-  - econstructor; eauto using live_exp_sound_incl.
-    etransitivity; eauto.
-  - econstructor; eauto. intros. edestruct H3; eauto.
-    destruct i; simpl; eauto; cset_tac.
-    cset_tac.
-Qed.
-
-(** ** Live variables always contain the free variables *)
 
 Lemma incl_incl_minus X `{OrderedType X} s t u v
   : t \ u ⊆ v -> s ⊆ t -> s \ u ⊆ v.
@@ -156,56 +115,62 @@ Qed.
 
 Hint Resolve incl_incl_minus incl_minus_exp_live_union : cset.
 
-Lemma freeVars_live s lv Lv
-  : live_sound Functional Lv s lv -> IL.freeVars s ⊆ getAnn lv.
+Hint Resolve incl_minus_lr : cset.
+
+Lemma live_sound_monotone i ZL LV LV' s lv
+: live_sound i ZL LV s lv
+  -> PIR2 Subset LV' LV
+  -> live_sound i ZL LV' s lv.
+Proof.
+  intros. general induction H; simpl; eauto using live_sound.
+  - PIR2_inv.
+    econstructor; eauto.
+    cases; eauto with cset.
+  - econstructor; eauto using PIR2_app.
+Qed.
+
+Lemma live_sound_monotone2 i ZL LV s lv a
+: live_sound i ZL LV s lv
+  -> getAnn lv ⊆ a
+  -> live_sound i ZL LV s (setTopAnn lv a).
+Proof.
+  intros. general induction H; simpl in * |- *;
+            eauto using live_sound, live_exp_sound_incl, Subset_trans with cset.
+  - econstructor; eauto using live_exp_sound_incl.
+    cases; eauto with cset.
+  - econstructor; eauto with cset.
+    + intros. edestruct H3; eauto.
+      cases; eauto with cset.
+Qed.
+
+(** ** Live variables always contain the free variables *)
+
+Lemma freeVars_live_list Y lv
+  : (forall (n : nat) (y : exp), get Y n y -> live_exp_sound y lv)
+    -> list_union (Exp.freeVars ⊝ Y) ⊆ lv.
+Proof.
+  intros H. eapply list_union_incl; intros; inv_get; eauto using Exp.freeVars_live.
+Qed.
+
+Lemma freeVars_live s lv ZL Lv
+  : live_sound Functional ZL Lv s lv -> IL.freeVars s ⊆ getAnn lv.
 Proof.
   intros.
-  induction H; simpl.
-  - eauto using Exp.freeVars_live with cset.
-  - eauto using Exp.freeVars_live with cset.
-  - eapply list_union_incl; eauto.
-    intros. inv_map H3.
-    eauto using Exp.freeVars_live with cset.
-  - eauto using Exp.freeVars_live with cset.
-  - rewrite (list_union_incl (s':=lv)); eauto with cset.
-    intros ? ? GET. inv_map GET.
-    eauto using Exp.freeVars_live with cset.
-  - eapply union_subset_3.
-    + eapply list_union_incl; intros; eauto.
-      inv_map H5. edestruct (get_length_eq _ H6 H0); eauto.
-      edestruct H3; eauto. simpl in *. exploit H2; eauto.
+  Start Profiling.
+  induction H; simpl; eauto using Exp.freeVars_live, freeVars_live_list with cset.
+  - eapply union_subset_3; eauto with cset.
+    + eapply list_union_incl; intros; inv_get; eauto.
+
+
+      edestruct H3; eauto; simpl in *. exploit H2; eauto.
       eauto with cset.
-    + rewrite IHlive_sound; eauto.
 Qed.
 
 (** ** Liveness is stable under renaming *)
 
-Definition live_rename_L_entry (ϱ:env var) (x:set var * params)
- := (lookup_set ϱ (fst x), lookup_list ϱ (snd x)).
-
-Definition live_rename_L (ϱ:env var) DL
-  := List.map (live_rename_L_entry ϱ) DL.
-
-Lemma live_rename_L_globals ϱ als F
-: length F = length als
-  -> live_rename_L ϱ (zip pair (getAnn ⊝ als) (fst ⊝ F)) =
-    zip pair
-        (getAnn ⊝ (List.map (mapAnn (lookup_set ϱ)) als))
-        (fst ⊝ (List.map (fun Zs0 => (lookup_list ϱ (fst Zs0), rename ϱ (snd Zs0))) F)).
-Proof.
-  intros. length_equify. general induction H; simpl; eauto.
-  - f_equal; eauto. rewrite getAnn_mapAnn; reflexivity.
-Qed.
-
-Lemma live_rename_L_app ϱ L L'
-: live_rename_L ϱ (L ++ L') = live_rename_L ϱ L ++ live_rename_L ϱ L'.
-Proof.
-  unfold live_rename_L. rewrite map_app; reflexivity.
-Qed.
-
-Lemma live_rename_sound i DL s an (ϱ:env var)
-: live_sound i DL s an
-  -> live_sound i (live_rename_L ϱ DL) (rename ϱ s) (mapAnn (lookup_set ϱ) an).
+Lemma live_rename_sound i ZL Lv s an (ϱ:env var)
+: live_sound i ZL Lv s an
+  -> live_sound i (lookup_list ϱ ⊝ ZL) (lookup_set ϱ ⊝ Lv) (rename ϱ s) (mapAnn (lookup_set ϱ) an).
 Proof.
   intros. general induction H; simpl.
   - econstructor; eauto using live_exp_rename_sound.
@@ -218,36 +183,32 @@ Proof.
   - econstructor; eauto using live_exp_rename_sound.
     + rewrite getAnn_mapAnn. eapply lookup_set_incl; eauto.
     + rewrite getAnn_mapAnn. eapply lookup_set_incl; eauto.
-  - pose proof (map_get_1 (live_rename_L_entry ϱ) H).
-    econstructor; eauto.
-    + destruct i; simpl in * |- *; eauto.
+  - econstructor; eauto with len.
+    + cases; eauto.
       rewrite of_list_lookup_list; eauto.
-      eapply Subset_trans. eapply lookup_set_minus_incl; eauto.
-      eapply lookup_set_incl; eauto. simpl.
-      rewrite of_list_lookup_list; eauto.
-      eapply Subset_trans. eapply lookup_set_minus_incl; eauto.
+      etransitivity. eapply lookup_set_minus_incl; eauto.
       eapply lookup_set_incl; eauto.
-    + simpl.
-      repeat rewrite lookup_list_length; eauto. rewrite map_length; eauto.
-    + intros. edestruct map_get_4; eauto; dcr; subst.
-      eapply live_exp_rename_sound; eauto.
+    + rewrite lookup_list_length; eauto with len.
+    + intros; inv_get; eauto using live_exp_rename_sound.
   - econstructor; eauto using live_exp_rename_sound.
-  - econstructor; intros; eauto using live_exp_rename_sound.
-    + edestruct map_get_4; eauto; dcr; subst.
-      eapply live_exp_rename_sound; eauto.
+  - econstructor; eauto using live_exp_rename_sound.
+    + intros; inv_get; eauto using live_exp_rename_sound.
     + rewrite getAnn_mapAnn.
       rewrite lookup_set_minus_single_incl; eauto.
       eapply lookup_set_incl; eauto.
     + rewrite getAnn_mapAnn; eauto. eapply lookup_set_spec; eauto.
-  - econstructor; eauto; try rewrite getAnn_mapAnn; eauto.
-    + rewrite <- live_rename_L_globals, <- live_rename_L_app; eauto.
-    + repeat rewrite map_length; eauto.
-    + intros. inv_map H5. inv_map H6.
-      rewrite <- live_rename_L_globals, <- live_rename_L_app; eauto.
-      eapply H2; eauto.
-    + intros. inv_map H6; inv_map H5.
+  - econstructor; eauto; try rewrite getAnn_mapAnn; eauto with len.
+    + repeat rewrite map_map; simpl. rewrite <- map_map.
+      rewrite <- map_app.
+      setoid_rewrite getAnn_mapAnn.
+      setoid_rewrite <- map_map at 3. rewrite <- map_app. eauto.
+    + intros; inv_get. simpl.
+      repeat rewrite map_map; simpl. rewrite <- map_map.
+      rewrite <- map_app.
+      setoid_rewrite getAnn_mapAnn.
+      setoid_rewrite <- map_map at 3. rewrite <- map_app. eauto.
+    + intros; inv_get; simpl.
       exploit H3; eauto; dcr. simpl.
-      assert (Proper (_eq ==> _eq) ϱ) by eapply Proper_eq_fun.
       split.
       * rewrite of_list_lookup_list; eauto.
         rewrite getAnn_mapAnn.
